### Section 7.2 Integration By Parts
p512: 1, 7, 9, 11, 13, 15, 17, 19, 23, 25, 27, 31, 33, 35,37, 40, 47, 51, 56, 60a

1\. On which derivative rule is integration by parts based?
>**Solution**
Product rule.

7-22\. **Integration by parts** Evaluate the following integrals.
7\. $\int x\cos x dx$
>**Solution**
$$
\eqalign{
u = x, &du = dx\\
dv = \cos x dx, &v = \sin x\\
\int x\cos x dx &= x\sin x - \int \sin x dx\\
&= x\sin x + \cos x + C
}
$$

9\. $\int t e^t dt$
>**Solution**
$$
\eqalign{
u = t, &du = dt\\
dv = e^t dt, &v = e^t\\
\int t e^t dt &= t e^t - \int e^t dt\\
&= t e^t - e^t + C
}
$$

11\. $\int \frac{x}{\sqrt {x+1}} dx$
>**Solution**
$$
\eqalign{
u = x, & du = dx\\
dv = \frac{1}{\sqrt {x+1}} dx, & v= 2\sqrt{x+1}\\
\int \frac{x}{\sqrt {x+1}} dx &= 2x\sqrt{x+1} - \int 2\sqrt{x+1} dx\\
&= 2x\sqrt{x+1} - -\frac{4}{3} (x+1)^{\frac{3}{2}} + C
}
$$

13\. $\int x^2\ln x dx$
>**Solution**
$$
\eqalign{
u = \ln x^3, & du = \frac{3}{x} dx\\
dv = x^2 dx, & v = \frac{1}{3}x^3\\
\int x^2\ln x^3dx &= \frac{1}{3}x^3 \ln x^3 - \int \frac{1}{3}x^3 \cdot \frac{3}{x} dx\\
&= x^3\ln x-\frac{1}{3}x^3 + C
}
$$

15\. $\int x^2\ln x dx$
>**Solution**
$$
\eqalign{
u = \ln x, & du = \frac{dx}{x}\\
dv = x^2 dx, & v = \frac{1}{3}x^3\\
\int x^2\ln x dx &= \frac{1}{3}x^3 \ln x - \int \frac{1}{3}x^3 \cdot \frac{1}{x} dx\\
&= \frac{1}{3}x^3\ln x-\frac{1}{9}x^3 + C
}
$$

17\. $\int \frac{\ln x}{x^{10}} dx$
>**Solution**
$$
\eqalign{
u = \ln x, & du = \frac{dx}{x}\\
dv = {x^{-10}} dx, &v = -\frac{1}{9} x^{-9}\\
\int \frac{\ln x}{x^{10}} dx &= -\frac{1}{9}x^{-9} \ln x - \int -\frac{1}{9} x^{-9} \frac{dx}{x}\\
&= -\frac{\ln x}{9x^9} - \frac{1}{81x^9} + C
}
$$

19\. $\int \arctan x dx$
>**Solution**
$$
\eqalign{
u = \arctan x, & du = \frac{dx}{1+x^2}\\
dv = dx, & v = x\\
\int \arctan x dx &= x\arctan x - \int x \cdot \frac{dx}{1+x^2}\\
&= x\arctan x - \frac{1}{2} \int \frac{1}{w} dw &( w=1+x^2, dw = 2xdx)\\
&= x\arctan x - \frac{1}{2}\ln (x^2+1) + C
}
$$

23\. $\int t^2 e^{-t} dt$
>**Solution**
$$
\eqalign{
u=t^2, & du = 2tdt\\
dv = e^{-t} dt, & v = -e^{-t}\\
\int t^2 e^{-t} dt &= -t^2 e^{-t} - \int -2t e^{-t} dt\\
&= -t^2 e^{-t} + 2\int t e^{-t} dt\\
&= -t^2 e^{-t} + 2(-t e^{-t} - \int -e^{-t} dt)\\
&= -t^2 e^{-t} - 2t e^{-t} - 2e^{-t} + C
}
$$

25\. $\int e^{-x} \sin 4x dx$
>**Solution**
$$
\eqalign{
u = \sin 4x, & du = 4\cos 4x dx\\
dv = e^{-x} dx, & v = -e^{-x}\\
\int e^{-x} \sin 4x dx &= -e^{-x}\sin 4x - \int -4 e^{-x} \cos 4x  dx\\
&= -e^{-x}\sin 4x + 4\int e^{-x} \cos 4x dx\\
u = \cos 4x, & du = -4\sin 4x dx\\
dv = e^{-x} dx, & v = -e^{-x}\\
&= -e^{-x}\sin 4x + 4(-e^{-x} \cos 4x - \int 4e^{-x} \sin 4x dx)\\
&= -e^{-x}\sin 4x - 4e^{-x} \cos 4x - 16 \int e^{-x} \sin 4x dx\\
17 \int e^{-x} \sin 4x dx &= -e^{-x}\sin 4x - 4e^{-x} \cos 4x\\
\int e^{-x} \sin 4x dx &= -\frac{1}{17} e^{-x}(\sin 4x + 4\cos 4x) + C
}
$$
